Imp Ch-12: add solutions of evaluating commands section

Imp.v
@@ -307,3 +307,355 @@ split.
 Qed.
 
 End AExp.
+
+Module aevalR_division.
+
+Inductive aexp : Type :=
+  | ANum (n : nat)
+  | APlus (a1 a2 : aexp)
+  | AMinus (a1 a2 : aexp)
+  | AMult (a1 a2 : aexp)
+  | ADiv (a1 a2 : aexp). (* <--- NEW *)
+
+Reserved Notation "e '\\' n"
+                  (at level 90, left associativity).
+Inductive aevalR : aexp -> nat -> Prop :=
+  | E_ANum (n : nat) :
+      (ANum n) \\ n
+  | E_APlus (a1 a2 : aexp) (n1 n2 : nat) :
+      (a1 \\ n1) -> (a2 \\ n2) -> (APlus a1 a2) \\ (n1 + n2)
+  | E_AMinus (a1 a2 : aexp) (n1 n2 : nat) :
+      (a1 \\ n1) -> (a2 \\ n2) -> (AMinus a1 a2) \\ (n1 - n2)
+  | E_AMult (a1 a2 : aexp) (n1 n2 : nat) :
+      (a1 \\ n1) -> (a2 \\ n2) -> (AMult a1 a2) \\ (n1 * n2)
+  | E_ADiv (a1 a2 : aexp) (n1 n2 n3 : nat) :
+      (a1 \\ n1) -> (a2 \\ n2) -> (n2 > 0) ->
+      (mult n2 n3 = n1) -> (ADiv a1 a2) \\ n3
+
+where "a '\\' n" := (aevalR a n) : type_scope.
+End aevalR_division.
+
+Module aevalR_extended.
+
+Reserved Notation "e '\\' n" (at level 90, left associativity).
+Inductive aexp : Type :=
+  | AAny (* <--- NEW *)
+  | ANum (n : nat)
+  | APlus (a1 a2 : aexp)
+  | AMinus (a1 a2 : aexp)
+  | AMult (a1 a2 : aexp).
+
+Inductive aevalR : aexp -> nat -> Prop :=
+  | E_Any (n : nat) :
+      AAny \\ n (* <--- NEW *)
+  | E_ANum (n : nat) :
+      (ANum n) \\ n
+  | E_APlus (a1 a2 : aexp) (n1 n2 : nat) :
+      (a1 \\ n1) -> (a2 \\ n2) -> (APlus a1 a2) \\ (n1 + n2)
+  | E_AMinus (a1 a2 : aexp) (n1 n2 : nat) :
+      (a1 \\ n1) -> (a2 \\ n2) -> (AMinus a1 a2) \\ (n1 - n2)
+  | E_AMult (a1 a2 : aexp) (n1 n2 : nat) :
+      (a1 \\ n1) -> (a2 \\ n2) -> (AMult a1 a2) \\ (n1 * n2)
+
+where "a '\\' n" := (aevalR a n) : type_scope.
+End aevalR_extended.
+
+(* Expressions With Variables *)
+
+Definition state := total_map nat.
+
+Inductive aexp : Type :=
+| ANum (n : nat)
+| AId (x : string)
+| APlus (a1 a2 : aexp)
+| AMinus (a1 a2 : aexp)
+| AMult (a1 a2 : aexp).
+
+Definition W : string := "W".
+Definition X : string := "X".
+Definition Y : string := "Y".
+Definition Z : string := "Z".
+
+Inductive bexp : Type :=
+| BTrue
+| BFalse
+| BEq (a1 a2 : aexp)
+| BLe (a1 a2 : aexp)
+| BNot (b : bexp)
+| BAnd (b1 b2 : bexp).
+
+Coercion AId : string >-> aexp.
+Coercion ANum : nat >-> aexp.
+
+Definition bool_to_bexp (b : bool) : bexp :=
+if b then BTrue else BFalse.
+Coercion bool_to_bexp : bool >-> bexp.
+
+Bind Scope imp_scope with aexp.
+Bind Scope imp_scope with bexp.
+Delimit Scope imp_scope with imp.
+
+Notation "x + y" := (APlus x y) (at level 50, left associativity) : imp_scope.
+Notation "x - y" := (AMinus x y) (at level 50, left associativity) : imp_scope.
+Notation "x * y" := (AMult x y) (at level 40, left associativity) : imp_scope.
+Notation "x <= y" := (BLe x y) (at level 70, no associativity) : imp_scope.
+Notation "x = y" := (BEq x y) (at level 70, no associativity) : imp_scope.
+Notation "x && y" := (BAnd x y) (at level 40, left associativity) : imp_scope.
+Notation "'~' b" := (BNot b) (at level 75, right associativity) : imp_scope.
+
+
+
+Definition example_aexp := (3 + (X * 2))%imp : aexp.
+Definition example_bexp := (true && ~(X <= 4))%imp : bexp.
+
+Set Printing Coercions.
+
+Print example_bexp.
+(* ===> example_bexp = bool_to_bexp true && ~ (AId X <= ANum 4) *)
+Unset Printing Coercions.
+
+Fixpoint aeval (st : state) (a : aexp) : nat :=
+match a with
+| ANum n => n
+| AId x => st x
+| APlus a1 a2 => (aeval st a1) + (aeval st a2)
+| AMinus a1 a2  => (aeval st a1) - (aeval st a2)
+| AMult a1 a2 => (aeval st a1) * (aeval st a2)
+end.
+
+Fixpoint beval (st : state) (b : bexp) : bool :=
+match b with
+| BTrue       => true
+| BFalse      => false
+| BEq a1 a2   => (aeval st a1) =? (aeval st a2)
+| BLe a1 a2   => (aeval st a1) <=? (aeval st a2)
+| BNot b1     => negb (beval st b1)
+| BAnd b1 b2  => andb (beval st b1) (beval st b2)
+end.
+
+Definition empty_st := (_ !-> 0).
+
+Notation "a '!->' x" := (t_update empty_st a x) (at level 100).
+
+Example aexp1 :
+aeval (X !-> 5) (3 + (X * 2))%imp
+= 13.
+Proof. reflexivity. Qed.
+
+Example bexp1 :
+beval (X !-> 5) (true && ~(X <= 4))%imp
+= true.
+Proof. reflexivity. Qed.
+
+(* Commands *)
+
+Inductive com : Type :=
+  | CSkip
+  | CAss (x : string) (a : aexp)
+  | CSeq (c1 c2 : com)
+  | CIf (b : bexp) (c1 c2 : com)
+  | CWhile (b : bexp) (c : com).
+
+Bind Scope imp_scope with com.
+Notation "'SKIP'" :=
+   CSkip : imp_scope.
+Notation "x '::=' a" :=
+  (CAss x a) (at level 60) : imp_scope.
+Notation "c1 ;; c2" :=
+  (CSeq c1 c2) (at level 80, right associativity) : imp_scope.
+Notation "'WHILE' b 'DO' c 'END'" :=
+  (CWhile b c) (at level 80, right associativity) : imp_scope.
+Notation "'TEST' c1 'THEN' c2 'ELSE' c3 'FI'" :=
+  (CIf c1 c2 c3) (at level 80, right associativity) : imp_scope.
+
+Definition fact_in_coq : com :=
+  (Z ::= X;;
+  Y ::= 1;;
+  WHILE ~(Z = 0) DO
+    Y ::= Y * Z;;
+    Z ::= Z - 1
+  END)%imp.
+
+Unset Printing Notations.
+Print fact_in_coq.
+(* ===>
+   fact_in_coq =
+   CSeq (CAss Z X)
+        (CSeq (CAss Y (S O))
+              (CWhile (BNot (BEq Z O))
+                      (CSeq (CAss Y (AMult Y Z))
+                            (CAss Z (AMinus Z (S O))))))
+        : com *)
+Set Printing Notations.
+Set Printing Coercions.
+Print fact_in_coq.
+(* ===>
+   fact_in_coq =
+   (Z ::= AId X;;
+   Y ::= ANum 1;;
+   WHILE ~ (AId Z = ANum 0) DO
+     Y ::= AId Y * AId Z;;
+     Z ::= AId Z - ANum 1
+   END)%imp
+       : com *)
+Unset Printing Coercions.
+
+Locate "&&".
+(* ===>
+   Notation "x && y" := andb x y : bool_scope (default interpretation) *)
+Locate ";;".
+(* ===>
+   Notation "c1 ;; c2" := CSeq c1 c2 : imp_scope (default interpretation) *)
+Locate "WHILE".
+(* ===>
+   Notation "'WHILE' b 'DO' c 'END'" := CWhile b c : imp_scope
+   (default interpretation) *)
+
+Locate aexp.
+(* ===>
+   Inductive Top.aexp
+   Inductive Top.AExp.aexp
+     (shorter name to refer to it in current context is AExp.aexp)
+   Inductive Top.aevalR_division.aexp
+     (shorter name to refer to it in current context is aevalR_division.aexp)
+   Inductive Top.aevalR_extended.aexp
+     (shorter name to refer to it in current context is aevalR_extended.aexp)
+*)
+
+Definition plus2 : com :=
+  X ::= X + 2.
+
+Definition XtimesYinZ : com :=
+  Z ::= X * Y.
+
+Definition subtract_slowly_body : com :=
+  Z ::= Z - 1 ;;
+  X ::= X - 1.
+
+Definition subtract_slowly : com :=
+  (WHILE ~(X = 0) DO
+    subtract_slowly_body
+  END)%imp.
+
+Definition subtract_3_from_5_slowly : com :=
+  X ::= 3 ;;
+  Z ::= 5 ;;
+  subtract_slowly.
+
+Definition loop : com :=
+  WHILE true DO
+    SKIP
+  END.
+
+(* Evaluating Commands *)
+
+Open Scope imp_scope.
+Fixpoint ceval_fun_no_while (st : state) (c : com)
+                          : state :=
+  match c with
+    | SKIP =>
+        st
+    | x ::= a1 =>
+        (x !-> (aeval st a1) ; st)
+    | c1 ;; c2 =>
+        let st' := ceval_fun_no_while st c1 in
+        ceval_fun_no_while st' c2
+    | TEST b THEN c1 ELSE c2 FI =>
+        if (beval st b)
+          then ceval_fun_no_while st c1
+          else ceval_fun_no_while st c2
+    | WHILE b DO c END =>
+        st (* bogus *)
+  end.
+Close Scope imp_scope.
+
+Reserved Notation "st '=[' c ']=>' st'"
+                  (at level 40).
+
+Inductive ceval : com -> state -> state -> Prop :=
+  | E_Skip : forall st,
+      st =[ SKIP ]=> st
+  | E_Ass : forall st a1 n x,
+      aeval st a1 = n ->
+      st =[ x ::= a1 ]=> (x !-> n ; st)
+  | E_Seq : forall c1 c2 st st' st'',
+      st =[ c1 ]=> st' ->
+      st' =[ c2 ]=> st'' ->
+      st =[ c1 ;; c2 ]=> st''
+  | E_IfTrue : forall st st' b c1 c2,
+      beval st b = true ->
+      st =[ c1 ]=> st' ->
+      st =[ TEST b THEN c1 ELSE c2 FI ]=> st'
+  | E_IfFalse : forall st st' b c1 c2,
+      beval st b = false ->
+      st =[ c2 ]=> st' ->
+      st =[ TEST b THEN c1 ELSE c2 FI ]=> st'
+  | E_WhileFalse : forall b st c,
+      beval st b = false ->
+      st =[ WHILE b DO c END ]=> st
+  | E_WhileTrue : forall st st' st'' b c,
+      beval st b = true ->
+      st =[ c ]=> st' ->
+      st' =[ WHILE b DO c END ]=> st'' ->
+      st =[ WHILE b DO c END ]=> st''
+
+  where "st =[ c ]=> st'" := (ceval c st st').
+
+Example ceval_example1:
+  empty_st =[
+     X ::= 2;;
+     TEST X <= 1
+       THEN Y ::= 3
+       ELSE Z ::= 4
+     FI
+  ]=> (Z !-> 4 ; X !-> 2).
+Proof.
+  (* We must supply the intermediate state *)
+  apply E_Seq with (X !-> 2).
+  - (* assignment command *)
+    apply E_Ass. reflexivity.
+  - (* if command *)
+    apply E_IfFalse.
+    reflexivity.
+    apply E_Ass. reflexivity.
+Qed.
+
+Example ceval_example2:
+  empty_st =[
+    X ::= 0;; Y ::= 1;; Z ::= 2
+  ]=> (Z !-> 2 ; Y !-> 1 ; X !-> 0).
+Proof.
+apply E_Seq with (X !-> 0).
+- apply E_Ass. reflexivity.
+- apply E_Seq with (Y !-> 1; X !-> 0).
+  + apply E_Ass. reflexivity.
+  + apply E_Ass. reflexivity.
+Qed.
+
+Definition pup_to_n : com :=
+Y ::= 0 ;;
+  WHILE ~ (X = 0) DO
+    Y ::= Y + X ;;
+    X ::= X - 1
+  END.
+
+Theorem pup_to_2_ceval :
+  (X !-> 2) =[
+    pup_to_n
+  ]=> (X !-> 0 ; Y !-> 3 ; X !-> 1 ; Y !-> 2 ; Y !-> 0 ; X !-> 2).
+Proof.
+unfold pup_to_n.
+apply E_Seq with (Y !-> 0; X !-> 2).
+- apply E_Ass. reflexivity.
+- apply E_WhileTrue with (X !-> 1; Y !-> 2; Y !-> 0; X !-> 2).
+  + reflexivity.
+  + apply E_Seq with (Y !-> 2; Y !-> 0; X !-> 2);  apply E_Ass. reflexivity.
+    * reflexivity.
+  + apply E_WhileTrue with (X !-> 0 ; Y !-> 3 ; X !-> 1; Y !-> 2; Y !-> 0; X !-> 2).
+    * reflexivity.
+    * apply E_Seq with (Y !-> 3; X !-> 1; Y !-> 2; Y !-> 0; X !-> 2); apply E_Ass. reflexivity.
+    reflexivity.
+    * apply E_WhileFalse.
+    reflexivity.
+Qed.
+
